@prefix : <http://iot-platform#> .
@prefix dc: <http://purl.org/dc/elements/1.1/> .
@prefix qu: <http://purl.org/NET/ssnx/qu/qu#> .
@prefix DUL: <http://www.loa-cnr.it/ontologies/DUL.owl#> .
@prefix dct: <http://purl.org/dc/terms/> .
@prefix geo: <http://www.w3.org/2003/01/geo/wgs84_pos#> .
@prefix owl: <http://www.w3.org/2002/07/owl#> .
@prefix rdf: <http://www.w3.org/1999/02/22-rdf-syntax-ns#> .
@prefix ssn: <http://purl.oclc.org/NET/ssnx/ssn#> .
@prefix xml: <http://www.w3.org/XML/1998/namespace> .
@prefix xsd: <http://www.w3.org/2001/XMLSchema#> .
@prefix foaf: <http://xmlns.com/foaf/0.1/> .
@prefix rdfs: <http://www.w3.org/2000/01/rdf-schema#> .
@prefix skos: <http://www.w3.org/2004/02/skos/core#> .
@prefix time: <http://www.w3.org/2006/time#> .
@prefix iot-lite: <http://purl.oclc.org/NET/UNIS/fiware/iot-lite#> .

<http://iot-platform> a owl:Ontology ;
	rdfs:label "iot-platform" .
# 
# 
# #################################################################
# #
# #    Annotation properties
# #
# #################################################################
# 
# 
# http://www.w3.org/2000/01/rdf-schema#comment

rdfs:comment a owl:AnnotationProperty .
# 
# http://www.w3.org/2000/01/rdf-schema#isDefinedBy

rdfs:isDefinedBy a owl:AnnotationProperty .
# 
# http://www.w3.org/2000/01/rdf-schema#label

rdfs:label a owl:AnnotationProperty .
# 
# http://www.w3.org/2000/01/rdf-schema#seeAlso

rdfs:seeAlso a owl:AnnotationProperty .
# 
# http://www.w3.org/2003/06/sw-vocab-status/ns#term_status

<http://www.w3.org/2003/06/sw-vocab-status/ns#term_status> a owl:AnnotationProperty .
# 
# 
# 
# #################################################################
# #
# #    Object Properties
# #
# #################################################################
# 
# 
# http://iot-platform#adminOf

:adminOf a owl:ObjectProperty ;
	rdfs:domain :Admin ;
	rdfs:range :Application ;
	rdfs:comment "It describes the relation between admin and application" .
# 
# http://iot-platform#developedApplication

:developedApplication a owl:ObjectProperty ;
	rdfs:domain :Developer ;
	rdfs:range :Application ;
	rdfs:comment "It describes the relation between a developer and the application he/she is developing ." .
# 
# http://iot-platform#hasDevice

:hasDevice a owl:ObjectProperty ;
	rdfs:domain :DeviceModule ;
	rdfs:range ssn:Device .
# 
# http://iot-platform#hasDeviceModule

:hasDeviceModule a owl:ObjectProperty ;
	rdfs:domain :IOTSystem ;
	rdfs:range :DeviceModule ;
	rdfs:comment "Describes the relation between an IOTSystem and DeviceModule." ;
	rdfs:label "has Device Module" .
# 
# http://iot-platform#hasService

:hasService a owl:ObjectProperty ;
	rdfs:domain ssn:Device ;
	rdfs:range iot-lite:Service ;
	rdfs:comment "A device has a service." .
# 
# http://iot-platform#usesApplication

:usesApplication a owl:ObjectProperty ;
	rdfs:domain :NormalUser ;
	rdfs:range :Application ;
	rdfs:comment "It specify the relation between a normal use (ie: cutomer) and application used by him/her ." .
# 
# http://iot-platform#usesSystem

:usesSystem a owl:ObjectProperty ;
	rdfs:domain :Application ;
	rdfs:range :IOTSystem ;
	rdfs:comment "It describes the relation that an IOT application uses a system (smart campus)" .
# 
# http://purl.oclc.org/NET/UNIS/fiware/iot-lite#hasAttribute

iot-lite:hasAttribute a owl:ObjectProperty ;
	rdfs:domain iot-lite:Object ;
	rdfs:range iot-lite:Attribute ;
	rdfs:comment "Links an Object with their attributes." .
# 
# http://purl.oclc.org/NET/UNIS/fiware/iot-lite#hasCoverage

iot-lite:hasCoverage a owl:ObjectProperty ;
	rdfs:domain ssn:Device ;
	rdfs:range iot-lite:Coverage ;
	rdfs:comment "Links the devices with their coverages." .
# 
# http://purl.oclc.org/NET/UNIS/fiware/iot-lite#hasMetadata

iot-lite:hasMetadata a owl:ObjectProperty ;
	rdfs:range iot-lite:Metadata ;
	rdfs:comment "Links any concept with metadata about that concept." .
# 
# http://purl.oclc.org/NET/UNIS/fiware/iot-lite#hasQuantityKind

iot-lite:hasQuantityKind a owl:ObjectProperty ;
	rdfs:domain iot-lite:Attribute , ssn:Sensor ;
	rdfs:range qu:QuantityKind ;
	rdfs:comment "Links a sensor or an attribute with the quantity  kind it measures (e.g. A sensor -sensor1- measures temperature: sensor1 hasQuantityKind temperature)." .
# 
# http://purl.oclc.org/NET/UNIS/fiware/iot-lite#hasSensingDevice

iot-lite:hasSensingDevice a owl:ObjectProperty ;
	rdfs:domain ssn:Sensor ;
	rdfs:range ssn:SensingDevice ;
	rdfs:comment "It describes the relation that a device can has attached snesing device (sensor) . ie: A module (device) has sensing device Tempreture sensor (sensing device )attached to it ." .
# 
# http://purl.oclc.org/NET/UNIS/fiware/iot-lite#hasUnit

iot-lite:hasUnit a owl:ObjectProperty ;
	rdfs:range qu:Unit ;
	rdfs:comment "Links the sensor with the units of the quantity kind it measures (e.g. A sensor -sensor1- measures temperature in Celsius: senso1 hasUnit celsius)." .
# 
# http://purl.oclc.org/NET/UNIS/fiware/iot-lite#isAssociatedWith

iot-lite:isAssociatedWith a owl:ObjectProperty ;
	rdfs:domain iot-lite:Object ;
	rdfs:range iot-lite:Service ;
	rdfs:comment "Defines the associations between objects and sensors (e.g. A table (object) has an attribute (temperature at the table) which is associated with a sensor (the temperature sensor of the room). " .
# 
# http://purl.oclc.org/NET/ssnx/ssn#deployedOnPlatform

ssn:deployedOnPlatform a owl:ObjectProperty ;
	rdfs:comment "Relation between a deployment and the platform on which the system was deployed." ;
	rdfs:isDefinedBy "http://purl.oclc.org/NET/ssnx/ssn" ;
	rdfs:label "deployed on platform" ;
	rdfs:seeAlso "http://www.w3.org/2005/Incubator/ssn/wiki/SSN_Deploy#Deployment" .
# 
# http://purl.oclc.org/NET/ssnx/ssn#deploymentProcessPart

ssn:deploymentProcessPart a owl:ObjectProperty ;
	rdfs:comment """Has part relation between a deployment process and its constituent processes.

It says that a ssn:deploymentProcess is part of another ssn:deploymentProcess""" ;
	rdfs:isDefinedBy "http://purl.oclc.org/NET/ssnx/ssn" ;
	rdfs:label "deployment process part" ;
	rdfs:seeAlso "http://www.w3.org/2005/Incubator/ssn/wiki/SSN_Deploy#Deployment" .
# 
# http://purl.oclc.org/NET/ssnx/ssn#detects

ssn:detects a owl:ObjectProperty ;
	rdfs:comment """A relation from a sensor to the Stimulus that the sensor can detect.   
The Stimulus itself will be serving as a proxy for (see isProxyOf) some observable property.""" ;
	rdfs:isDefinedBy "http://purl.oclc.org/NET/ssnx/ssn" ;
	rdfs:label "detects" ;
	rdfs:seeAlso "http://www.w3.org/2005/Incubator/ssn/wiki/SSN_Skeleton#Skeleton" .
# 
# http://purl.oclc.org/NET/ssnx/ssn#featureOfInterest

ssn:featureOfInterest a owl:ObjectProperty ;
	rdfs:comment "A relation between an observation and the entity whose quality was observed.   For example, in an observation of the weight of a person, the feature of interest is the person and the quality is weight." ;
	rdfs:isDefinedBy "http://purl.oclc.org/NET/ssnx/ssn" ;
	rdfs:label "feature of interest" ;
	rdfs:seeAlso "http://www.w3.org/2005/Incubator/ssn/wiki/SSN_Skeleton#Skeleton" .
# 
# http://purl.oclc.org/NET/ssnx/ssn#forProperty

ssn:forProperty a owl:ObjectProperty ;
	rdfs:comment """A relation between some aspect of a sensing entity and a property.  For example, from a sensor to the properties it can observe, or from a deployment to the properties it was installed to observe.  Also from a measurement capability to the property the capability is described for.  (Used in conjunction with ofFeature).

A ssn:MeasurementCapability is something that is a ssn:Property and has a ssn:hasMeasurementProperty property who must be a ssn:MeasurementProperty . 

So ssn:MeasurementCapability instance will have a ssn:forProperty property who must be a ssn:Property and has a ssn:inCondition property who must be a ssn:Condition""" ;
	rdfs:isDefinedBy "http://purl.oclc.org/NET/ssnx/ssn" ;
	rdfs:label "for property" ;
	rdfs:seeAlso "http://www.w3.org/2005/Incubator/ssn/wiki/SSN_Skeleton#Skeleton" .
# 
# http://purl.oclc.org/NET/ssnx/ssn#hasDeployment

ssn:hasDeployment a owl:ObjectProperty ;
	rdfs:comment "Relation between a System and a Deployment, recording that the System/Sensor was deployed in that Deployment." ;
	rdfs:isDefinedBy "http://purl.oclc.org/NET/ssnx/ssn" ;
	rdfs:label "has deployment" ;
	rdfs:seeAlso "http://www.w3.org/2005/Incubator/ssn/wiki/SSN_Deploy#Deployment" .
# 
# http://purl.oclc.org/NET/ssnx/ssn#hasInput

ssn:hasInput a owl:ObjectProperty ;
	rdfs:isDefinedBy "http://purl.oclc.org/NET/ssnx/ssn" ;
	rdfs:label "has input" ;
	rdfs:seeAlso "http://www.w3.org/2005/Incubator/ssn/wiki/SSN_Model#Process" .
# 
# http://purl.oclc.org/NET/ssnx/ssn#hasMeasurementCapability

ssn:hasMeasurementCapability a owl:ObjectProperty ;
	rdfs:subPropertyOf ssn:hasProperty ;
	rdfs:comment "Relation from a Sensor to a MeasurementCapability describing the measurement properties of the sensor." ;
	rdfs:isDefinedBy "http://purl.oclc.org/NET/ssnx/ssn" ;
	rdfs:label "has measurement  capability" ;
	rdfs:seeAlso "http://www.w3.org/2005/Incubator/ssn/wiki/SSN_Sensor#MeasuringCapability" .
# 
# http://purl.oclc.org/NET/ssnx/ssn#hasMeasurementProperty

ssn:hasMeasurementProperty a owl:ObjectProperty ;
	rdfs:subPropertyOf ssn:hasProperty ;
	rdfs:comment "Relation from a MeasurementCapability to a MeasurementProperty.  For example, to an accuracy (see notes at MeasurementCapability)." ;
	rdfs:isDefinedBy "http://purl.oclc.org/NET/ssnx/ssn" ;
	rdfs:label "has measurement property" ;
	rdfs:seeAlso "http://www.w3.org/2005/Incubator/ssn/wiki/SSN_Sensor#MeasuringCapability" .
# 
# http://purl.oclc.org/NET/ssnx/ssn#hasOperatingProperty

ssn:hasOperatingProperty a owl:ObjectProperty ;
	rdfs:subPropertyOf ssn:hasProperty ;
	rdfs:comment "Relation from an OperatingRange to a Property.  For example, to a battery lifetime." ;
	rdfs:isDefinedBy "http://purl.oclc.org/NET/ssnx/ssn" ;
	rdfs:label "has operating property" ;
	rdfs:seeAlso "http://www.w3.org/2005/Incubator/ssn/wiki/SSN_Deploy#OperatingRestriction" .
# 
# http://purl.oclc.org/NET/ssnx/ssn#hasOperatingRange

ssn:hasOperatingRange a owl:ObjectProperty ;
	rdfs:subPropertyOf ssn:hasProperty ;
	rdfs:comment "Relation from a System to an OperatingRange describing the normal operating environment of the System." ;
	rdfs:isDefinedBy "http://purl.oclc.org/NET/ssnx/ssn" ;
	rdfs:label "has operating range" ;
	rdfs:seeAlso "http://www.w3.org/2005/Incubator/ssn/wiki/SSN_Deploy#OperatingRestriction" .
# 
# http://purl.oclc.org/NET/ssnx/ssn#hasOutput

ssn:hasOutput a owl:ObjectProperty ;
	rdfs:isDefinedBy "http://purl.oclc.org/NET/ssnx/ssn" ;
	rdfs:label "has output" ;
	rdfs:seeAlso "http://www.w3.org/2005/Incubator/ssn/wiki/SSN_Model#Process" .
# 
# http://purl.oclc.org/NET/ssnx/ssn#hasProperty

ssn:hasProperty a owl:ObjectProperty ;
	rdfs:comment "A relation between a FeatureOfInterest and a Property of that feature. A FeatureOfInterest can have more than one property." ;
	rdfs:isDefinedBy "http://purl.oclc.org/NET/ssnx/ssn" ;
	rdfs:label "has property" ;
	rdfs:seeAlso "http://www.w3.org/2005/Incubator/ssn/wiki/SSN_Skeleton#Skeleton" .
# 
# http://purl.oclc.org/NET/ssnx/ssn#hasSubSystem

ssn:hasSubSystem a owl:ObjectProperty ;
	rdfs:domain ssn:System ;
	rdfs:range ssn:System ;
	rdfs:comment "Haspart relation between a system and its parts." ;
	rdfs:isDefinedBy "http://purl.oclc.org/NET/ssnx/ssn" ;
	rdfs:label "has subsystem" ;
	rdfs:seeAlso "http://www.w3.org/2005/Incubator/ssn/wiki/SSN_Model#System" .
# 
# http://purl.oclc.org/NET/ssnx/ssn#hasSurvivalProperty

ssn:hasSurvivalProperty a owl:ObjectProperty ;
	rdfs:subPropertyOf ssn:hasProperty ;
	rdfs:comment "Relation from a SurvivalRange to a Property describing the survial range of a system.  For example, to the temperature extreme that a system can withstand before being considered damaged." ;
	rdfs:isDefinedBy "http://purl.oclc.org/NET/ssnx/ssn" ;
	rdfs:label "has survival property" ;
	rdfs:seeAlso "http://www.w3.org/2005/Incubator/ssn/wiki/SSN_Deploy#OperatingRestriction" .
# 
# http://purl.oclc.org/NET/ssnx/ssn#hasSurvivalRange

ssn:hasSurvivalRange a owl:ObjectProperty ;
	rdfs:subPropertyOf ssn:hasProperty ;
	rdfs:comment "A Relation from a System to a SurvivalRange." ;
	rdfs:isDefinedBy "http://purl.oclc.org/NET/ssnx/ssn" ;
	rdfs:label "has survival range" ;
	rdfs:seeAlso "http://www.w3.org/2005/Incubator/ssn/wiki/SSN_Deploy#OperatingRestriction" .
# 
# http://purl.oclc.org/NET/ssnx/ssn#hasValue

ssn:hasValue a owl:ObjectProperty ;
	rdfs:isDefinedBy "http://purl.oclc.org/NET/ssnx/ssn" ;
	rdfs:label "has value" ;
	rdfs:seeAlso "http://www.w3.org/2005/Incubator/ssn/wiki/SSN_Base#Data" .
# 
# http://purl.oclc.org/NET/ssnx/ssn#implements

ssn:implements a owl:ObjectProperty ;
	rdfs:comment "A relation between an entity that implements a method in some executable way and the description of an algorithm, procedure or method.  For example, between a Sensor and the scientific measuring method that the Sensor uses to observe a Property." ;
	rdfs:isDefinedBy "http://purl.oclc.org/NET/ssnx/ssn" ;
	rdfs:label "implements" ;
	rdfs:seeAlso "http://www.w3.org/2005/Incubator/ssn/wiki/SSN_Skeleton#Skeleton" .
# 
# http://purl.oclc.org/NET/ssnx/ssn#inCondition

ssn:inCondition a owl:ObjectProperty ;
	rdfs:comment "Describes the prevailing environmental conditions for MeasurementCapabilites, OperatingConditions and SurvivalRanges.  Used for example to say that a sensor has a particular accuracy in particular conditions.  (see also MeasurementCapability)" ;
	rdfs:isDefinedBy "http://purl.oclc.org/NET/ssnx/ssn" ;
	rdfs:label "in condition" ;
	rdfs:seeAlso "http://www.w3.org/2005/Incubator/ssn/wiki/SSN_Base#ConstraintBlock" .
# 
# http://purl.oclc.org/NET/ssnx/ssn#isProducedBy

ssn:isProducedBy a owl:ObjectProperty ;
	rdfs:comment "Relation between a producer and a produced entity: for example, between a sensor and the produced output." ;
	rdfs:isDefinedBy "http://purl.oclc.org/NET/ssnx/ssn" ;
	rdfs:label "is produced by" ;
	rdfs:seeAlso "http://www.w3.org/2005/Incubator/ssn/wiki/SSN_Model#Process" .
# 
# http://purl.oclc.org/NET/ssnx/ssn#isProxyFor

ssn:isProxyFor a owl:ObjectProperty ;
	rdfs:comment """A relation from a Stimulus to the Property that the Stimulus is serving as a proxy for.

For example, the expansion of the quicksilver is a stimulus that serves as a proxy for temperature, or an increase or decrease in the spinning of cups on a wind sensor is serving as a proxy for wind speed.""" ;
	rdfs:isDefinedBy "http://purl.oclc.org/NET/ssnx/ssn" ;
	rdfs:label "isProxyFor" ;
	rdfs:seeAlso "http://www.w3.org/2005/Incubator/ssn/wiki/SSN_Skeleton#Skeleton" .
# 
# http://purl.oclc.org/NET/ssnx/ssn#observationResult

ssn:observationResult a owl:ObjectProperty ;
	rdfs:comment "Relation linking an Observation (i.e., a description of the context, the Situation, in which the observatioin was made) and a Result(Sensor Output), which contains a value representing the value associated with the observed Property." ;
	rdfs:isDefinedBy "http://purl.oclc.org/NET/ssnx/ssn" ;
	rdfs:label "observation result" ;
	rdfs:seeAlso "http://www.w3.org/2005/Incubator/ssn/wiki/SSN_Skeleton#Skeleton" .
# 
# http://purl.oclc.org/NET/ssnx/ssn#observedProperty

ssn:observedProperty a owl:ObjectProperty ;
	rdfs:comment "Relation linking an Observation to the Property that was observed.  The observedProperty should be a Property (hasProperty) of the FeatureOfInterest (linked by featureOfInterest) of this observation." ;
	rdfs:isDefinedBy "http://purl.oclc.org/NET/ssnx/ssn" ;
	rdfs:label "observed property" ;
	rdfs:seeAlso "http://www.w3.org/2005/Incubator/ssn/wiki/SSN_Skeleton#Skeleton" .
# 
# http://purl.oclc.org/NET/ssnx/ssn#observes

ssn:observes a owl:ObjectProperty ;
	rdfs:comment "Relation between a Sensor and a Property that the sensor can observe. It points to a property observed by a sensor (e.g., temperature, acceleration, wind speed)." ;
	rdfs:isDefinedBy "http://purl.oclc.org/NET/ssnx/ssn" ;
	rdfs:label "observes" ;
	rdfs:seeAlso "http://www.w3.org/2005/Incubator/ssn/wiki/SSN_Sensor#Measuring" .
# 
# http://purl.oclc.org/NET/ssnx/ssn#onPlatform

ssn:onPlatform a owl:ObjectProperty ;
	rdfs:domain ssn:System ;
	rdfs:range ssn:Platform ;
	rdfs:comment "Relation between a System (e.g., a Sensor) and a Platform.  The relation locates the sensor relative to other described entities entities: i.e., the Sensor s1's location is Platform p1.  More precise locations for sensors in space (relative to other entities, where attached to another entity, or in 3D space) are made using DOLCE's Regions (SpaceRegion)." ;
	rdfs:isDefinedBy "http://purl.oclc.org/NET/ssnx/ssn" ;
	rdfs:label "on platform" ;
	rdfs:seeAlso "http://www.w3.org/2005/Incubator/ssn/wiki/SSN_Deploy#PlatformSite" .
# 
# http://purl.oclc.org/NET/ssnx/ssn#sensingMethodUsed

ssn:sensingMethodUsed a owl:ObjectProperty ;
	rdfs:comment "A (measurement) procedure is a detailed description of a measurement according to one or more measurement principles and to a given measurement method, based on a measurement model and including any calculation to obtain a measurement result [VIM 2.6]" ;
	rdfs:isDefinedBy "http://purl.oclc.org/NET/ssnx/ssn" ;
	rdfs:label "sensing method used" ;
	rdfs:seeAlso "http://www.w3.org/2005/Incubator/ssn/wiki/SSN_Skeleton#Skeleton" .
# 
# http://www.loa-cnr.it/ontologies/DUL.owl#includesEvent

DUL:includesEvent a owl:ObjectProperty ;
	rdfs:comment "Links an observation to its stimulus(Event)." .
# 
# http://www.w3.org/2003/01/geo/wgs84_pos#hasLocation

geo:hasLocation a owl:ObjectProperty ;
	rdfs:range geo:Point .
# 
# http://xmlns.com/foaf/0.1/fundedBy

foaf:fundedBy a owl:ObjectProperty ;
	rdfs:domain :Application ;
	rdfs:range foaf:Organization ;
	rdfs:comment "An organization funding a project or person." ;
	rdfs:isDefinedBy "http://xmlns.com/foaf/0.1/" ;
	rdfs:label "funded by" .
# 
# http://xmlns.com/foaf/0.1/knows

foaf:knows a owl:ObjectProperty ;
	rdfs:domain foaf:Person ;
	rdfs:range foaf:Person ;
	rdfs:comment "A person known by this person (indicating some level of reciprocated interaction between the parties)." ;
	rdfs:isDefinedBy <http://xmlns.com/foaf/0.1/> ;
	rdfs:label "knows" ;
	<http://www.w3.org/2003/06/sw-vocab-status/ns#term_status> "stable" .
# 
# http://xmlns.com/foaf/0.1/member

foaf:member a owl:ObjectProperty ;
	rdfs:domain foaf:Group ;
	rdfs:range foaf:Agent ;
	rdfs:comment "Indicates a member of a Group" ;
	rdfs:isDefinedBy <http://xmlns.com/foaf/0.1/> ;
	rdfs:label "member" ;
	<http://www.w3.org/2003/06/sw-vocab-status/ns#term_status> "stable" .
# 
# 
# 
# #################################################################
# #
# #    Data properties
# #
# #################################################################
# 
# 
# http://iot-platform#description

:description a owl:DatatypeProperty ;
	rdfs:range xsd:string ;
	rdfs:comment "Description of a thing" .
# 
# http://iot-platform#dutyCycle

:dutyCycle a owl:DatatypeProperty ;
	rdfs:range xsd:string ;
	rdfs:comment "Describes the duty cycle of a communicating device." ;
	rdfs:label "Duty Cycle" .
# 
# http://iot-platform#hasBandwidth

:hasBandwidth a owl:DatatypeProperty ;
	rdfs:domain :CommunicatingDevice ;
	rdfs:range xsd:double ;
	rdfs:comment "Describes the bandwidth of a communicating device." .
# 
# http://iot-platform#hasDataValue

:hasDataValue a owl:DatatypeProperty ;
	rdfs:domain :Amount ;
	rdfs:range xsd:double ;
	rdfs:comment "Describes the value of an amount . ie: the value of property like frequency or senstivity or batteryLifeTime" .
# 
# http://iot-platform#hasFrequency

:hasFrequency a owl:DatatypeProperty ;
	rdfs:domain :CommunicatingDevice ;
	rdfs:range xsd:double ;
	rdfs:comment "Describes the frequency of transmission of a communictating device" .
# 
# http://iot-platform#hasNetworkTopology

:hasNetworkTopology a owl:DatatypeProperty ;
	rdfs:domain :CommunicatingDevice ;
	rdfs:range xsd:string ;
	rdfs:comment "Describes the network topology of a communicating device" .
# 
# http://iot-platform#hasRangeMaxValue

:hasRangeMaxValue a owl:DatatypeProperty ;
	rdfs:domain :Amount ;
	rdfs:range xsd:double ;
	rdfs:comment "It describes the max value amount of a range of a property like operatingPowerRange" .
# 
# http://iot-platform#hasRangeMinValue

:hasRangeMinValue a owl:DatatypeProperty ;
	rdfs:domain :Amount ;
	rdfs:range xsd:double ;
	rdfs:comment "It describes the min value amount of a range of a property like operatingPowerRange" .
# 
# http://iot-platform#hasTransmissionPower

:hasTransmissionPower a owl:DatatypeProperty ;
	rdfs:domain :CommunicatingDevice ;
	rdfs:range xsd:double ;
	rdfs:comment "Describes the transmission power of a communicating device" .
# 
# http://iot-platform#hasType

:hasType a owl:DatatypeProperty ;
	rdfs:domain :CommunicatingDevice ;
	rdfs:range xsd:string ;
	rdfs:comment "Describes the type of a communicating device ie: BLE ." .
# 
# http://iot-platform#rangeOfTransmission

:rangeOfTransmission a owl:DatatypeProperty ;
	rdfs:subPropertyOf owl:topDataProperty ;
	rdfs:range xsd:string ;
	rdfs:comment "Describes the range of transmission of a communicating device." ;
	rdfs:label "Range of transmission" .
# 
# http://purl.oclc.org/NET/UNIS/fiware/iot-lite#endpoint

iot-lite:endpoint a owl:DatatypeProperty ;
	rdfs:domain iot-lite:Service ;
	rdfs:range xsd:anyURI ;
	rdfs:comment "Endpoint of a service (i.e. URL that provides a RESTful interface (website fo example to give more information about the service ) to access a service) ," .
# 
# http://purl.oclc.org/NET/UNIS/fiware/iot-lite#id

iot-lite:id a owl:DatatypeProperty ;
	rdfs:domain ssn:Device ;
	rdfs:range xsd:string .
# 
# http://purl.oclc.org/NET/UNIS/fiware/iot-lite#interfaceDescription

iot-lite:interfaceDescription a owl:DatatypeProperty ;
	rdfs:domain iot-lite:Service ;
	rdfs:range xsd:string ;
	rdfs:comment "Description of the service." .
# 
# http://purl.oclc.org/NET/UNIS/fiware/iot-lite#interfaceType

iot-lite:interfaceType a owl:DatatypeProperty ;
	rdfs:domain iot-lite:Service ;
	rdfs:range xsd:string ;
	rdfs:comment "Defines the type of interface of the service endpoint." .
# 
# http://purl.oclc.org/NET/UNIS/fiware/iot-lite#isMobile

iot-lite:isMobile a owl:DatatypeProperty ;
	rdfs:domain ssn:Platform ;
	rdfs:range xsd:boolean ;
	rdfs:comment "Describes if the platform is moving . ie: fish (A fish is a type of platform because a sensor can be attached to it)" .
# 
# http://purl.oclc.org/NET/UNIS/fiware/iot-lite#metadataType

iot-lite:metadataType a owl:DatatypeProperty ;
	rdfs:domain iot-lite:Metadata ;
	rdfs:range xsd:string ;
	rdfs:comment "Defines the type pf the metadata value (e.g. resolution of the sensor)." .
# 
# http://purl.oclc.org/NET/UNIS/fiware/iot-lite#metadataValue

iot-lite:metadataValue a owl:DatatypeProperty ;
	rdfs:domain iot-lite:Metadata ;
	rdfs:range xsd:string ;
	rdfs:comment "Value of the metadata" .
# 
# http://purl.oclc.org/NET/UNIS/fiware/iot-lite#radius

iot-lite:radius a owl:DatatypeProperty ;
	rdfs:domain iot-lite:Circle ;
	rdfs:range xsd:double ;
	rdfs:comment "Specifies the radius of a circle coverage defined by a point -the center of the circle- and its radius." .
# 
# http://purl.oclc.org/NET/ssnx/ssn#endTime

ssn:endTime a owl:DatatypeProperty ;
	rdfs:range xsd:string ;
	rdfs:isDefinedBy "http://purl.oclc.org/NET/ssnx/ssn" ;
	rdfs:label "end time" ;
	rdfs:seeAlso "http://www.w3.org/2005/Incubator/ssn/wiki/SSN_Base#Time" .
# 
# http://purl.oclc.org/NET/ssnx/ssn#observationResultTime

ssn:observationResultTime a owl:DatatypeProperty ;
	rdfs:domain ssn:Observation ;
	rdfs:range xsd:string ;
	rdfs:comment "The result time is the time when the procedure associated with the observation act was applied." , "The result time shall describe the time when the result became available, typically when the procedure associated with the observation was completed For some observations this is identical to the phenomenonTime. However, there are important cases where they differ.[O&M]" ;
	rdfs:isDefinedBy "http://purl.oclc.org/NET/ssnx/ssn" ;
	rdfs:label "observation result time" ;
	rdfs:seeAlso "http://www.w3.org/2005/Incubator/ssn/wiki/SSN_Observation#Observation" .
# 
# http://purl.oclc.org/NET/ssnx/ssn#observationSamplingTime

ssn:observationSamplingTime a owl:DatatypeProperty ;
	rdfs:domain ssn:Observation ;
	rdfs:range xsd:string ;
	rdfs:comment "Rebadged as phenomenon time in [O&M]. The phenomenon time shall describe the time that the result applies to the property of the feature-of-interest. This is often the time of interaction by a sampling procedure or observation procedure with a real-world feature." , "The sampling time is the time that the result applies to the feature-of-interest. This is the time usually required for geospatial analysis of the result." ;
	rdfs:isDefinedBy "http://purl.oclc.org/NET/ssnx/ssn" ;
	rdfs:label "observation sampling time" ;
	rdfs:seeAlso "http://www.w3.org/2005/Incubator/ssn/wiki/SSN_Observation#Observation" .
# 
# http://purl.oclc.org/NET/ssnx/ssn#qualityOfObservation

ssn:qualityOfObservation a owl:DatatypeProperty ;
	rdfs:domain ssn:Observation ;
	rdfs:range xsd:double .
# 
# http://purl.oclc.org/NET/ssnx/ssn#startTime

ssn:startTime a owl:DatatypeProperty ;
	rdfs:range xsd:string ;
	rdfs:isDefinedBy "http://purl.oclc.org/NET/ssnx/ssn" ;
	rdfs:label "start time" ;
	rdfs:seeAlso "http://www.w3.org/2005/Incubator/ssn/wiki/SSN_Base#Time" .
# 
# http://www.w3.org/2003/01/geo/wgs84_pos#lat

geo:lat a owl:DatatypeProperty ;
	rdfs:domain geo:Point ;
	rdfs:range xsd:double ;
	rdfs:comment "Describes the value of latitude of a point" .
# 
# http://www.w3.org/2003/01/geo/wgs84_pos#long

geo:long a owl:DatatypeProperty ;
	rdfs:domain geo:Point ;
	rdfs:range xsd:double ;
	rdfs:comment "Describes the longtitude of a point" .
# 
# http://xmlns.com/foaf/0.1/age

foaf:age a owl:DatatypeProperty , owl:FunctionalProperty ;
	rdfs:domain foaf:Person ;
	rdfs:range rdfs:Literal ;
	rdfs:comment "The age in years of some agent." ;
	rdfs:isDefinedBy <http://xmlns.com/foaf/0.1/> ;
	rdfs:label "age" ;
	<http://www.w3.org/2003/06/sw-vocab-status/ns#term_status> "unstable" .
# 
# http://xmlns.com/foaf/0.1/birthday

foaf:birthday a owl:DatatypeProperty , owl:FunctionalProperty ;
	rdfs:domain foaf:Agent ;
	rdfs:range xsd:string ;
	rdfs:comment "The birthday of this Agent, represented in mm-dd string form, eg. '12-31'." ;
	rdfs:isDefinedBy <http://xmlns.com/foaf/0.1/> ;
	rdfs:label "birthday" ;
	<http://www.w3.org/2003/06/sw-vocab-status/ns#term_status> "unstable" .
# 
# http://xmlns.com/foaf/0.1/familyName

foaf:familyName a owl:DatatypeProperty ;
	rdfs:domain foaf:Person ;
	rdfs:range xsd:string ;
	rdfs:comment "The family name of some person." ;
	rdfs:isDefinedBy <http://xmlns.com/foaf/0.1/> ;
	rdfs:label "familyName" ;
	<http://www.w3.org/2003/06/sw-vocab-status/ns#term_status> "testing" .
# 
# http://xmlns.com/foaf/0.1/firstName

foaf:firstName a owl:DatatypeProperty ;
	rdfs:domain foaf:Person ;
	rdfs:range xsd:string ;
	rdfs:comment "The first name of a person." ;
	rdfs:isDefinedBy <http://xmlns.com/foaf/0.1/> ;
	rdfs:label "firstName" ;
	<http://www.w3.org/2003/06/sw-vocab-status/ns#term_status> "testing" .
# 
# http://xmlns.com/foaf/0.1/gender

foaf:gender a owl:DatatypeProperty , owl:FunctionalProperty ;
	rdfs:domain foaf:Agent ;
	rdfs:range xsd:string ;
	rdfs:comment "The gender of this Agent (typically but not necessarily 'male' or 'female')." ;
	rdfs:isDefinedBy <http://xmlns.com/foaf/0.1/> ;
	rdfs:label "gender" ;
	<http://www.w3.org/2003/06/sw-vocab-status/ns#term_status> "testing" .
# 
# http://xmlns.com/foaf/0.1/mbox

foaf:mbox a owl:DatatypeProperty ;
	rdfs:domain foaf:Agent ;
	rdfs:range xsd:string .
# 
# http://xmlns.com/foaf/0.1/middleName

foaf:middleName a owl:DatatypeProperty ;
	rdfs:domain foaf:Person ;
	rdfs:range xsd:string ;
	rdfs:comment "The last name of a person." ;
	rdfs:isDefinedBy <http://xmlns.com/foaf/0.1/> ;
	rdfs:label "middleName" ;
	<http://www.w3.org/2003/06/sw-vocab-status/ns#term_status> "testing" .
# 
# http://xmlns.com/foaf/0.1/name

foaf:name a owl:DatatypeProperty ;
	rdfs:domain owl:Thing ;
	rdfs:range xsd:string ;
	rdfs:comment "Describes the name of a thing. (eg: Application,Device)." ;
	rdfs:label "Name" .
# 
# http://xmlns.com/foaf/0.1/title

foaf:title a owl:DatatypeProperty ;
	rdfs:comment "Title (Mr, Mrs, Ms, Dr. etc)" ;
	rdfs:isDefinedBy <http://xmlns.com/foaf/0.1/> ;
	rdfs:label "title" ;
	<http://www.w3.org/2003/06/sw-vocab-status/ns#term_status> "testing" .
# 
# http://xmlns.com/foaf/0.1/topic_interest

foaf:topic_interest a owl:DatatypeProperty ;
	rdfs:domain foaf:Agent ;
	rdfs:range xsd:string ;
	rdfs:comment "A thing of interest to this person." ;
	rdfs:isDefinedBy <http://xmlns.com/foaf/0.1/> ;
	rdfs:label "topic of interest" .
# 
# http://xmlns.com/foaf/0.1/userName

foaf:userName a owl:DatatypeProperty ;
	rdfs:domain foaf:Person ;
	rdfs:range xsd:string ;
	rdfs:comment "Describes a unique user name of a user." ;
	rdfs:label "User Name" .
# 
# 
# 
# #################################################################
# #
# #    Classes
# #
# #################################################################
# 
# 
# http://iot-platform#Admin

:Admin a owl:Class ;
	rdfs:subClassOf foaf:Person ;
	rdfs:comment "Describes the admin of a system . This allows to specify certin privilages to that type of user" .
# 
# http://iot-platform#Amount

:Amount a owl:Class ;
	rdfs:comment "Describes the amount of of a ssn:MeasurementProperty or ssn:OperatingProperty" .
# 
# http://iot-platform#Application

:Application a owl:Class ;
	rdfs:comment "Describes an IOT Application deployed on the platform" .
# 
# http://iot-platform#CommunicatingDevice

:CommunicatingDevice a owl:Class ;
	rdfs:subClassOf ssn:Device ;
	rdfs:comment "Describes communicating device which allow communication of a device with the outer world . ie: Zegbee, BLE and WIFI" .
# 
# http://iot-platform#Developer

:Developer a owl:Class ;
	rdfs:subClassOf foaf:Person ;
	rdfs:comment "It describes the developer of an application. This allows to specify certin privilages to that type of user" .
# 
# http://iot-platform#DeviceModule

:DeviceModule a owl:Class ;
	rdfs:comment "DeviceModule is a module that consists of one or mix of devices (communicating Device, Tag Device, ActuatingDevice, CommunicatingDevice)" ;
	rdfs:label "Device Module" .
# 
# http://iot-platform#IOTSystem

:IOTSystem a owl:Class ;
	rdfs:comment "Describes an IOT system eg: Smart Campus, Smart City. The IOT System consists of one or more Device module." ;
	rdfs:label "IOT System" .
# 
# http://iot-platform#NormalUser

:NormalUser a owl:Class ;
	rdfs:subClassOf foaf:Person ;
	rdfs:comment "It describes a normal user who uses an application . ie: Customer . This allows to specify certin privilages to that type of user" .
# 
# http://purl.oclc.org/NET/UNIS/fiware/iot-lite#ActuatingDevice

iot-lite:ActuatingDevice a owl:Class ;
	rdfs:subClassOf ssn:Device ;
	rdfs:comment "Device that can actuate over an object or QuantityKind."@en .
# 
# http://purl.oclc.org/NET/UNIS/fiware/iot-lite#Attribute

iot-lite:Attribute a owl:Class ;
	rdfs:comment "An attribute of an IoT object that can be exposed by an IoT service (i.e. a room (IoT Object) has a temperature (Attribute), that can be exposed by a temperature sensor (IoT device)."@en .
# 
# http://purl.oclc.org/NET/UNIS/fiware/iot-lite#Circle

iot-lite:Circle a owl:Class ;
	rdfs:subClassOf iot-lite:Coverage ;
	rdfs:comment "Circle coverage it needs the location of the sensor as the centre of the circle and the radius as a DataProperty."@en .
# 
# http://purl.oclc.org/NET/UNIS/fiware/iot-lite#Coverage

iot-lite:Coverage a owl:Class ;
	rdfs:comment "The coverage of an IoT device (i.e. a temperature sensor inside a room has a coverage of that room)."@en .
# 
# http://purl.oclc.org/NET/UNIS/fiware/iot-lite#Metadata

iot-lite:Metadata a owl:Class ;
	rdfs:comment "Class used to describe properties that cannot be described by QuantityKind and Units. i.e. the resolution of a sensor."@en .
# 
# http://purl.oclc.org/NET/UNIS/fiware/iot-lite#Object

iot-lite:Object a owl:Class ;
	rdfs:comment "An Object or IoT entity that represent the place.  (i.e. room, car, table)"@en .
# 
# http://purl.oclc.org/NET/UNIS/fiware/iot-lite#Polygon

iot-lite:Polygon a owl:Class ;
	rdfs:subClassOf iot-lite:Coverage ;
	rdfs:comment "The coverage is made up by linking several points by strait lines."@en .
# 
# http://purl.oclc.org/NET/UNIS/fiware/iot-lite#Rectangle

iot-lite:Rectangle a owl:Class ;
	rdfs:subClassOf iot-lite:Coverage ;
	rdfs:comment "Teh coverage is made up by giving two points which are the oposite corners of a rentangle."@en .
# 
# http://purl.oclc.org/NET/UNIS/fiware/iot-lite#Service

iot-lite:Service a owl:Class ;
	rdfs:comment "Service provided by an IoT Device"@en .
# 
# http://purl.oclc.org/NET/UNIS/fiware/iot-lite#TagDevice

iot-lite:TagDevice a owl:Class ;
	rdfs:subClassOf ssn:Device ;
	rdfs:comment "Tag Device such as QR code or bar code."@en .
# 
# http://purl.oclc.org/NET/ssnx/ssn#Accuracy

ssn:Accuracy a owl:Class ;
	rdfs:subClassOf ssn:MeasurementProperty ;
	rdfs:comment "The closeness of agreement between the value of an observation and the true value of the observed quality." ;
	rdfs:isDefinedBy "http://purl.oclc.org/NET/ssnx/ssn" ;
	rdfs:label "Accuracy" ;
	rdfs:seeAlso "http://www.w3.org/2005/Incubator/ssn/wiki/SSN_Sensor#MeasuringCapability" .
# 
# http://purl.oclc.org/NET/ssnx/ssn#BatteryLifetime

ssn:BatteryLifetime a owl:Class ;
	rdfs:subClassOf ssn:SurvivalProperty ;
	rdfs:comment "Total useful life of a battery." ;
	rdfs:isDefinedBy "http://purl.oclc.org/NET/ssnx/ssn" ;
	rdfs:label "Battery Lifetime" ;
	rdfs:seeAlso "http://www.w3.org/2005/Incubator/ssn/wiki/SSN_Energy#EnergyRestriction" .
# 
# http://purl.oclc.org/NET/ssnx/ssn#Condition

ssn:Condition a owl:Class ;
	rdfs:subClassOf ssn:Property ;
	rdfs:comment "Used to specify ranges for qualities that act as conditions on a system/sensor's operation.  For example, wind speed of 10-60m/s is expressed as a condition linking a quality, wind speed, a unit of measurement, metres per second, and a set of values, 10-60, and may be used as the condition on a MeasurementProperty, for example, to state that a sensor has a particular accuracy in that condition." ;
	rdfs:isDefinedBy "http://purl.oclc.org/NET/ssnx/ssn" ;
	rdfs:label "Condition" ;
	rdfs:seeAlso "http://www.w3.org/2005/Incubator/ssn/wiki/SSN_Base#ConstraintBlock" .
# 
# http://purl.oclc.org/NET/ssnx/ssn#Deployment

ssn:Deployment a owl:Class ;
	rdfs:subClassOf ssn:DeploymentRelatedProcess , _:genid1 .

_:genid1 a owl:Restriction ;
	owl:onProperty ssn:deployedOnPlatform ;
	owl:allValuesFrom ssn:Platform .

ssn:Deployment rdfs:comment "The ongoing Process of Entities (for the purposes of this ontology, mainly sensors) deployed for a particular purpose.  For example, a particular Sensor deployed on a Platform, or a whole network of Sensors deployed for an observation campaign. The deployment may have sub processes, such as installation, maintenance, addition, and decomissioning and removal. It expresses the purpose of deployment not the service that the device offers ." ;
	rdfs:isDefinedBy "http://purl.oclc.org/NET/ssnx/ssn" ;
	rdfs:label "Deployment" ;
	rdfs:seeAlso "http://www.w3.org/2005/Incubator/ssn/wiki/SSN_Deploy#Deployment" .
# 
# http://purl.oclc.org/NET/ssnx/ssn#DeploymentRelatedProcess

ssn:DeploymentRelatedProcess a owl:Class ;
	rdfs:subClassOf _:genid2 .

_:genid2 a owl:Restriction ;
	owl:onProperty ssn:deploymentProcessPart ;
	owl:allValuesFrom ssn:DeploymentRelatedProcess .

ssn:DeploymentRelatedProcess rdfs:comment "Place to group all the various Processes related to Deployment.  For example, as well as Deplyment, installation, maintenance, deployment of further sensors and the like would all be classified under DeploymentRelatedProcess and it can link to deploymentRelatedProcess together using deploymentPorcessPart property ." ;
	rdfs:isDefinedBy "http://purl.oclc.org/NET/ssnx/ssn" ;
	rdfs:label "Deployment-related Process" ;
	rdfs:seeAlso "http://www.w3.org/2005/Incubator/ssn/wiki/SSN_Deploy#Deployment" .
# 
# http://purl.oclc.org/NET/ssnx/ssn#DetectionLimit

ssn:DetectionLimit a owl:Class ;
	rdfs:subClassOf ssn:MeasurementProperty ;
	rdfs:comment "An observed value for which the probability of falsely claiming the absence of a component in a material is Î², given a probability Î± of falsely claiming its presence." ;
	rdfs:isDefinedBy "http://purl.oclc.org/NET/ssnx/ssn" ;
	rdfs:label "detection limit" ;
	rdfs:seeAlso "http://www.w3.org/2005/Incubator/ssn/wiki/SSN_Sensor#MeasuringCapability" .
# 
# http://purl.oclc.org/NET/ssnx/ssn#Device

ssn:Device a owl:Class ;
	rdfs:subClassOf ssn:System ;
	rdfs:comment "A device is a physical piece of technology - a system in a box. Devices may of course be built of smaller devices and software components (i.e. systems have components)." ;
	rdfs:isDefinedBy "http://purl.oclc.org/NET/ssnx/ssn" ;
	rdfs:label "Device" ;
	rdfs:seeAlso "http://www.w3.org/2005/Incubator/ssn/wiki/SSN_Device#Device" .
# 
# http://purl.oclc.org/NET/ssnx/ssn#Drift

ssn:Drift a owl:Class ;
	rdfs:subClassOf ssn:MeasurementProperty ;
	rdfs:comment "A, continuous or incremental, change in the reported values of observations over time for an unchanging quality." ;
	rdfs:isDefinedBy "http://purl.oclc.org/NET/ssnx/ssn" ;
	rdfs:label "Drift" ;
	rdfs:seeAlso "http://www.w3.org/2005/Incubator/ssn/wiki/SSN_Sensor#MeasuringCapability" .
# 
# http://purl.oclc.org/NET/ssnx/ssn#FeatureOfInterest

ssn:FeatureOfInterest a owl:Class ;
	rdfs:subClassOf owl:Thing , _:genid3 .

_:genid3 a owl:Restriction ;
	owl:onProperty ssn:hasProperty ;
	owl:someValuesFrom ssn:Property .

ssn:FeatureOfInterest rdfs:subClassOf _:genid4 .

_:genid4 a owl:Restriction ;
	owl:onProperty ssn:hasProperty ;
	owl:allValuesFrom ssn:Property .

ssn:FeatureOfInterest rdfs:comment """A feature is an abstraction of real world phenomena (thing, person, event, etc) that are the target of sensing .

A relation between an observation and the entity whose quality was observed. For example, in an observation of the weight of a person, the feature of interest is the person and the quality is weight. A soil is a feature of interest has property soil tempreture and qualty is tempreture .

Features of interest can be events or objects but not qualities ex:  accuracy is not a property of a temperature but the property of a sensor or an observation procedure""" ;
	rdfs:isDefinedBy "http://purl.oclc.org/NET/ssnx/ssn" ;
	rdfs:label "Feature of Interest" ;
	rdfs:seeAlso "http://www.w3.org/2005/Incubator/ssn/wiki/SSN_Skeleton#Skeleton" .
# 
# http://purl.oclc.org/NET/ssnx/ssn#Frequency

ssn:Frequency a owl:Class ;
	rdfs:subClassOf ssn:MeasurementProperty ;
	rdfs:comment "The smallest possible time between one observation and the next." ;
	rdfs:isDefinedBy "http://purl.oclc.org/NET/ssnx/ssn" ;
	rdfs:label "Frequency" ;
	rdfs:seeAlso "http://www.w3.org/2005/Incubator/ssn/wiki/SSN_Sensor#MeasuringCapability" .
# 
# http://purl.oclc.org/NET/ssnx/ssn#Input

ssn:Input a owl:Class ;
	owl:disjointWith ssn:Output ;
	rdfs:comment "Any information that is provided to a process for its use [MMI OntDev]" ;
	rdfs:isDefinedBy "http://purl.oclc.org/NET/ssnx/ssn" ;
	rdfs:label "Input" ;
	rdfs:seeAlso "http://www.w3.org/2005/Incubator/ssn/wiki/SSN_Model#Process" .
# 
# http://purl.oclc.org/NET/ssnx/ssn#Latency

ssn:Latency a owl:Class ;
	rdfs:subClassOf ssn:MeasurementProperty ;
	rdfs:comment "The time between a request for an observation and the sensor providing a result." ;
	rdfs:isDefinedBy "http://purl.oclc.org/NET/ssnx/ssn" ;
	rdfs:label "Latency" ;
	rdfs:seeAlso "http://www.w3.org/2005/Incubator/ssn/wiki/SSN_Sensor#MeasuringCapability" .
# 
# http://purl.oclc.org/NET/ssnx/ssn#MaintenanceSchedule

ssn:MaintenanceSchedule a owl:Class ;
	rdfs:subClassOf ssn:OperatingProperty ;
	rdfs:comment "Schedule of maintenance for a system/sensor in the specified conditions." ;
	rdfs:isDefinedBy "http://purl.oclc.org/NET/ssnx/ssn" ;
	rdfs:label "Maintenance Schedule" ;
	rdfs:seeAlso "http://www.w3.org/2005/Incubator/ssn/wiki/SSN_Deploy#OperatingRestriction" .
# 
# http://purl.oclc.org/NET/ssnx/ssn#MeasurementCapability

ssn:MeasurementCapability a owl:Class ;
	rdfs:subClassOf ssn:Property , _:genid5 .

_:genid5 a owl:Restriction ;
	owl:onProperty ssn:forProperty ;
	owl:allValuesFrom ssn:Property .

ssn:MeasurementCapability rdfs:subClassOf _:genid6 .

_:genid6 a owl:Restriction ;
	owl:onProperty ssn:hasMeasurementProperty ;
	owl:allValuesFrom ssn:MeasurementProperty .

ssn:MeasurementCapability rdfs:subClassOf _:genid7 .

_:genid7 a owl:Restriction ;
	owl:onProperty ssn:inCondition ;
	owl:allValuesFrom ssn:Condition .

ssn:MeasurementCapability rdfs:comment """Collects together measurement properties (accuracy, range, precision, etc) and the environmental conditions in which those properties hold, representing a specification of a sensor's capability in those conditions.

One instance of ssn:MeasurementCapability can describe a set of measurement properties linked by the property ssn:hasMeasurementProperty and connected to a property using ssn:forProperty

A sensor can observe a number of PROPERTIES and this allows measurement capabilities to be defined for EACH property

The conditions, in which these measurement properties are valid, are specified using the property ssn:inCondition and expressed using an instance of the class ssn:Condition (i.e. observable conditions that affect the operation of the sensor)

ex: The sensor that measure acceleration has acceleration measurment capability""" ;
	rdfs:isDefinedBy "http://purl.oclc.org/NET/ssnx/ssn" ;
	rdfs:label "Measurement Capability" ;
	rdfs:seeAlso "http://www.w3.org/2005/Incubator/ssn/wiki/SSN_Sensor#MeasuringCapability" .
# 
# http://purl.oclc.org/NET/ssnx/ssn#MeasurementProperty

ssn:MeasurementProperty a owl:Class ;
	rdfs:subClassOf ssn:Property ;
	rdfs:comment "An identifiable and observable characteristic of a sensor's observations or ability to make observations." ;
	rdfs:isDefinedBy "http://purl.oclc.org/NET/ssnx/ssn" ;
	rdfs:label "Measurement  Property" ;
	rdfs:seeAlso "http://www.w3.org/2005/Incubator/ssn/wiki/SSN_Sensor#MeasuringCapability" .
# 
# http://purl.oclc.org/NET/ssnx/ssn#MeasurementRange

ssn:MeasurementRange a owl:Class ;
	rdfs:subClassOf ssn:MeasurementProperty ;
	rdfs:comment "The set of values that the sensor can return as the result of an observation under the defined conditions with the defined measurement properties.  (If no conditions are specified or the conditions do not specify a range for the observed qualities, the measurement range is to be taken as the condition for the observed qualities.)" ;
	rdfs:isDefinedBy "http://purl.oclc.org/NET/ssnx/ssn" ;
	rdfs:label "Measurement  Range" ;
	rdfs:seeAlso "http://www.w3.org/2005/Incubator/ssn/wiki/SSN_Sensor#MeasuringCapability" .
# 
# http://purl.oclc.org/NET/ssnx/ssn#Observation

ssn:Observation a owl:Class ;
	rdfs:subClassOf _:genid8 .

_:genid8 a owl:Restriction ;
	owl:onProperty DUL:includesEvent ;
	owl:someValuesFrom ssn:Stimulus .

ssn:Observation rdfs:subClassOf _:genid9 .

_:genid9 a owl:Restriction ;
	owl:onProperty ssn:featureOfInterest ;
	owl:allValuesFrom ssn:FeatureOfInterest .

ssn:Observation rdfs:subClassOf _:genid10 .

_:genid10 a owl:Restriction ;
	owl:onProperty ssn:observationResult ;
	owl:allValuesFrom ssn:SensorOutput .

ssn:Observation rdfs:subClassOf _:genid11 .

_:genid11 a owl:Restriction ;
	owl:onProperty ssn:observedProperty ;
	owl:allValuesFrom ssn:Property .

ssn:Observation rdfs:subClassOf _:genid12 .

_:genid12 a owl:Restriction ;
	owl:onProperty ssn:sensingMethodUsed ;
	owl:allValuesFrom ssn:Sensing .

ssn:Observation rdfs:subClassOf _:genid13 .

_:genid13 a owl:Restriction ;
	owl:onProperty ssn:featureOfInterest ;
	owl:qualifiedCardinality "1"^^xsd:nonNegativeInteger ;
	owl:onClass ssn:FeatureOfInterest .

ssn:Observation rdfs:subClassOf _:genid14 .

_:genid14 a owl:Restriction ;
	owl:onProperty ssn:observedProperty ;
	owl:qualifiedCardinality "1"^^xsd:nonNegativeInteger ;
	owl:onClass ssn:Property .

ssn:Observation rdfs:subClassOf _:genid15 .

_:genid15 a owl:Restriction ;
	owl:onProperty ssn:sensingMethodUsed ;
	owl:qualifiedCardinality "1"^^xsd:nonNegativeInteger ;
	owl:onClass ssn:Sensing .

ssn:Observation rdfs:subClassOf _:genid16 .

_:genid16 a owl:Restriction ;
	owl:onProperty ssn:observationResultTime ;
	owl:minCardinality "0"^^xsd:nonNegativeInteger .

ssn:Observation rdfs:subClassOf _:genid17 .

_:genid17 a owl:Restriction ;
	owl:onProperty ssn:observationSamplingTime ;
	owl:minCardinality "0"^^xsd:nonNegativeInteger .

ssn:Observation rdfs:comment "An Observation is made by a sensor and it is a Situation in which a Sensing method has been used to estimate or calculate a value of a Property of a FeatureOfInterest.  Links to Sensing and Sensor describe what made the Observation and how; links to Property and Feature detail what was sensed; the result is the output of a Sensor; other metadata details times etc." ;
	rdfs:isDefinedBy "http://purl.oclc.org/NET/ssnx/ssn" ;
	rdfs:label "Observation" ;
	rdfs:seeAlso "http://www.w3.org/2005/Incubator/ssn/wiki/SSN_Skeleton#Skeleton" .
# 
# http://purl.oclc.org/NET/ssnx/ssn#ObservationValue

ssn:ObservationValue a owl:Class ;
	rdfs:comment "The value of the result of an Observation.  An Observation has a result which is the output of some sensor, the result is an information object that encodes some value for a Feature." ;
	rdfs:isDefinedBy "http://purl.oclc.org/NET/ssnx/ssn" ;
	rdfs:label "Observation Value" ;
	rdfs:seeAlso "http://www.w3.org/2005/Incubator/ssn/wiki/SSN_Base#Data" .
# 
# http://purl.oclc.org/NET/ssnx/ssn#OperatingPowerRange

ssn:OperatingPowerRange a owl:Class ;
	rdfs:subClassOf ssn:OperatingProperty ;
	rdfs:comment "Power range in which system/sensor is expected to operate." ;
	rdfs:isDefinedBy "http://purl.oclc.org/NET/ssnx/ssn" ;
	rdfs:label "Operating Power Range" ;
	rdfs:seeAlso "http://www.w3.org/2005/Incubator/ssn/wiki/SSN_Energy#EnergyRestriction" .
# 
# http://purl.oclc.org/NET/ssnx/ssn#OperatingProperty

ssn:OperatingProperty a owl:Class ;
	rdfs:subClassOf ssn:Property ;
	rdfs:comment "An identifiable characteristic of the environmental and other conditions in which the sensor is intended to operate.  May include power ranges, power sources, standard configurations, attachments and the like." ;
	rdfs:isDefinedBy "http://purl.oclc.org/NET/ssnx/ssn" ;
	rdfs:label "Operating Property" ;
	rdfs:seeAlso "http://www.w3.org/2005/Incubator/ssn/wiki/SSN_Deploy#OperatingRestriction" .
# 
# http://purl.oclc.org/NET/ssnx/ssn#OperatingRange

ssn:OperatingRange a owl:Class ;
	rdfs:subClassOf ssn:Property , _:genid18 .

_:genid18 a owl:Restriction ;
	owl:onProperty ssn:hasOperatingProperty ;
	owl:allValuesFrom ssn:OperatingProperty .

ssn:OperatingRange rdfs:subClassOf _:genid19 .

_:genid19 a owl:Restriction ;
	owl:onProperty ssn:inCondition ;
	owl:allValuesFrom ssn:Condition .

ssn:OperatingRange rdfs:comment """The environmental conditions and characteristics of a system/sensor's normal operating environment.  Can be used to specify for example the standard environmental conditions in which the sensor is expected to operate (a Condition with no OperatingProperty), or how the environmental and other operating properties relate: i.e., that the maintenance schedule or power requirements differ according to the conditions. 

If the Operating Range exceeded ,the system must be maintained""" ;
	rdfs:isDefinedBy "http://purl.oclc.org/NET/ssnx/ssn" ;
	rdfs:label "Operating Range" ;
	rdfs:seeAlso "http://www.w3.org/2005/Incubator/ssn/wiki/SSN_Deploy#OperatingRestriction" .
# 
# http://purl.oclc.org/NET/ssnx/ssn#Output

ssn:Output a owl:Class ;
	rdfs:comment "Any information that is reported from a process. [MMI OntDev]" ;
	rdfs:isDefinedBy "http://purl.oclc.org/NET/ssnx/ssn" ;
	rdfs:label "Output" ;
	rdfs:seeAlso "http://www.w3.org/2005/Incubator/ssn/wiki/SSN_Model#Process" .
# 
# http://purl.oclc.org/NET/ssnx/ssn#Platform

ssn:Platform a owl:Class ;
	rdfs:comment "An Entity to which other Entities can be attached - particuarly Sensors and other Platforms.  For example, a post might act as the Platform, a bouy might act as a Platform, or a fish might act as a Platform for an attached sensor." ;
	rdfs:isDefinedBy "http://purl.oclc.org/NET/ssnx/ssn" ;
	rdfs:label "Platform" ;
	rdfs:seeAlso "http://www.w3.org/2005/Incubator/ssn/wiki/SSN_Deploy#PlatformSite" .
# 
# http://purl.oclc.org/NET/ssnx/ssn#Precision

ssn:Precision a owl:Class ;
	rdfs:subClassOf ssn:MeasurementProperty ;
	rdfs:comment "The closeness of agreement between replicate observations on an unchanged or similar quality value: i.e., a measure of a sensor's ability to consitently reproduce an observation." ;
	rdfs:isDefinedBy "http://purl.oclc.org/NET/ssnx/ssn" ;
	rdfs:label "Precision" ;
	rdfs:seeAlso "http://www.w3.org/2005/Incubator/ssn/wiki/SSN_Sensor#MeasuringCapability" .
# 
# http://purl.oclc.org/NET/ssnx/ssn#Process

ssn:Process a owl:Class ;
	rdfs:subClassOf _:genid20 .

_:genid20 a owl:Restriction ;
	owl:onProperty ssn:hasOutput ;
	owl:someValuesFrom ssn:Output .

ssn:Process rdfs:subClassOf _:genid21 .

_:genid21 a owl:Restriction ;
	owl:onProperty ssn:hasInput ;
	owl:allValuesFrom ssn:Input .

ssn:Process rdfs:subClassOf _:genid22 .

_:genid22 a owl:Restriction ;
	owl:onProperty ssn:hasOutput ;
	owl:allValuesFrom ssn:Output .

ssn:Process rdfs:comment "A process has an output and possibly inputs and, for a composite process, describes the temporal and dataflow dependencies and relationships amongst its parts. [SSN XG]" ;
	rdfs:isDefinedBy "http://purl.oclc.org/NET/ssnx/ssn" ;
	rdfs:label "Process" ;
	rdfs:seeAlso "http://www.w3.org/2005/Incubator/ssn/wiki/SSN_Model#Process" .
# 
# http://purl.oclc.org/NET/ssnx/ssn#Property

ssn:Property a owl:Class ;
	rdfs:comment "An observable Quality of an Event or Object.  That is, not a quality of an abstract entity as is also allowed by DUL's Quality, but rather an aspect of an entity that is intrinsic to and cannot exist without the entity and is observable by a sensor." ;
	rdfs:isDefinedBy "http://purl.oclc.org/NET/ssnx/ssn" ;
	rdfs:label "Property" ;
	rdfs:seeAlso "http://www.w3.org/2005/Incubator/ssn/wiki/SSN_Skeleton#Skeleton" .
# 
# http://purl.oclc.org/NET/ssnx/ssn#Resolution

ssn:Resolution a owl:Class ;
	rdfs:subClassOf ssn:MeasurementProperty ;
	rdfs:comment "The smallest difference in the value of a quality being observed that would result in perceptably different values of observation results." ;
	rdfs:isDefinedBy "http://purl.oclc.org/NET/ssnx/ssn" ;
	rdfs:label "Resolution" ;
	rdfs:seeAlso "http://www.w3.org/2005/Incubator/ssn/wiki/SSN_Sensor#MeasuringCapability" .
# 
# http://purl.oclc.org/NET/ssnx/ssn#ResponseTime

ssn:ResponseTime a owl:Class ;
	rdfs:subClassOf ssn:MeasurementProperty ;
	rdfs:comment "The time between a (step) change inthe value of an observed quality and a sensor (possibly with specified error) 'settling' on an observed value." ;
	rdfs:isDefinedBy "http://purl.oclc.org/NET/ssnx/ssn" ;
	rdfs:label "Response time" ;
	rdfs:seeAlso "http://www.w3.org/2005/Incubator/ssn/wiki/SSN_Sensor#MeasuringCapability" .
# 
# http://purl.oclc.org/NET/ssnx/ssn#Selectivity

ssn:Selectivity a owl:Class ;
	rdfs:subClassOf ssn:MeasurementProperty ;
	rdfs:comment "Selectivity is a property of a sensor whereby it provides observed values for one or more qualities such that the values of each quality are independent of other qualities in the phenomenon, body, or substance being investigated." ;
	rdfs:isDefinedBy "http://purl.oclc.org/NET/ssnx/ssn" ;
	rdfs:label "Selectivity" ;
	rdfs:seeAlso "http://www.w3.org/2005/Incubator/ssn/wiki/SSN_Sensor#MeasuringCapability" .
# 
# http://purl.oclc.org/NET/ssnx/ssn#Sensing

ssn:Sensing a owl:Class ;
	rdfs:subClassOf ssn:Process ;
	rdfs:comment """Sensing is a process that results in the estimation, or calculation, of the value of a phenomenon.

Defining the specification of the procedure implemented in a sensor. It may be specified as a known principle or method or, if a computer science approach is followed, as a function which has an output and possibly some inputs. which is expressed using ssn:hasInput and ssn:hasOutput properties""" ;
	rdfs:isDefinedBy "http://purl.oclc.org/NET/ssnx/ssn" ;
	rdfs:label "Sensing" ;
	rdfs:seeAlso "http://www.w3.org/2005/Incubator/ssn/wiki/SSN_Skeleton#Skeleton" .
# 
# http://purl.oclc.org/NET/ssnx/ssn#SensingDevice

ssn:SensingDevice a owl:Class ;
	rdfs:subClassOf ssn:Sensor ;
	rdfs:comment "A sensing device is a device that implements sensing." ;
	rdfs:isDefinedBy "http://purl.oclc.org/NET/ssnx/ssn" ;
	rdfs:label "Sensing Device" ;
	rdfs:seeAlso "http://www.w3.org/2005/Incubator/ssn/wiki/SSN_Sensor#Measuring" .
# 
# http://purl.oclc.org/NET/ssnx/ssn#Sensitivity

ssn:Sensitivity a owl:Class ;
	rdfs:subClassOf ssn:MeasurementProperty ;
	rdfs:comment "Sensitivity is the quotient of the change in a result of sensor and the corresponding change in a value of a quality being observed." ;
	rdfs:isDefinedBy "http://purl.oclc.org/NET/ssnx/ssn" ;
	rdfs:label "Sensitivity" ;
	rdfs:seeAlso "http://www.w3.org/2005/Incubator/ssn/wiki/SSN_Sensor#MeasuringCapability" .
# 
# http://purl.oclc.org/NET/ssnx/ssn#Sensor

ssn:Sensor a owl:Class ;
	rdfs:subClassOf ssn:Device , _:genid23 .

_:genid23 a owl:Restriction ;
	owl:onProperty ssn:implements ;
	owl:someValuesFrom ssn:Sensing .

ssn:Sensor rdfs:subClassOf _:genid24 .

_:genid24 a owl:Restriction ;
	owl:onProperty ssn:detects ;
	owl:allValuesFrom ssn:Stimulus .

ssn:Sensor rdfs:subClassOf _:genid25 .

_:genid25 a owl:Restriction ;
	owl:onProperty ssn:hasMeasurementCapability ;
	owl:allValuesFrom ssn:MeasurementCapability .

ssn:Sensor rdfs:subClassOf _:genid26 .

_:genid26 a owl:Restriction ;
	owl:onProperty ssn:observes ;
	owl:allValuesFrom ssn:Property .

ssn:Sensor rdfs:comment "A sensor can do (implements) sensing: that is, a sensor is any entity that can follow a sensing method and thus observe some Property of a FeatureOfInterest.  Sensors may be physical devices, computational methods, a laboratory setup with a person following a method, or any other thing that can follow a Sensing Method to observe a Property." ;
	rdfs:isDefinedBy "http://purl.oclc.org/NET/ssnx/ssn" ;
	rdfs:label "Sensor" ;
	rdfs:seeAlso "http://www.w3.org/2005/Incubator/ssn/wiki/SSN_Skeleton#Skeleton" .
# 
# http://purl.oclc.org/NET/ssnx/ssn#SensorDataSheet

ssn:SensorDataSheet a owl:Class ;
	rdfs:comment """A data sheet records properties of a sensor.  A data sheet might describe for example the accuracy in various conditions, the power use, the types of connectors that the sensor has, etc.  

Generally a sensor's properties are recorded directly (with hasMeasurementCapability, for example), but the data sheet can be used for example to record the manufacturers specifications verses observed capabilites, or if more is known than the manufacturer specifies, etc.  The data sheet is an information object about the sensor's properties, rather than a direct link to the actual properties themselves.""" ;
	rdfs:isDefinedBy "http://purl.oclc.org/NET/ssnx/ssn" ;
	rdfs:label "Sensor Data Sheet" ;
	rdfs:seeAlso "http://www.w3.org/2005/Incubator/ssn/wiki/SSN_Sensor#Measuring" .
# 
# http://purl.oclc.org/NET/ssnx/ssn#SensorOutput

ssn:SensorOutput a owl:Class ;
	rdfs:subClassOf _:genid27 .

_:genid27 a owl:Restriction ;
	owl:onProperty ssn:hasValue ;
	owl:someValuesFrom ssn:ObservationValue .

ssn:SensorOutput rdfs:subClassOf _:genid28 .

_:genid28 a owl:Restriction ;
	owl:onProperty ssn:isProducedBy ;
	owl:someValuesFrom ssn:Sensor .

ssn:SensorOutput rdfs:comment "A sensor outputs a piece of information (an observed value), the value itself being represented by an ObservationValue." ;
	rdfs:isDefinedBy "http://purl.oclc.org/NET/ssnx/ssn" ;
	rdfs:label "Sensor Output" ;
	rdfs:seeAlso "http://www.w3.org/2005/Incubator/ssn/wiki/SSN_Skeleton#Skeleton" .
# 
# http://purl.oclc.org/NET/ssnx/ssn#Stimulus

ssn:Stimulus a owl:Class ;
	rdfs:subClassOf _:genid29 .

_:genid29 a owl:Restriction ;
	owl:onProperty ssn:isProxyFor ;
	owl:allValuesFrom ssn:Property .

ssn:Stimulus rdfs:comment """An Event in the real world that 'triggers' the sensor.  The properties associated to the stimulus may be different to eventual observed property.  It is the event, not the object that triggers the sensor.

Based on the work of Quine, the skeleton defines stimuli as the (only) link to the physical environment. Empirical science observes these stimuli using sensors to infer information about environmental properties and construct features of interest.

Stimuli are detectable changes in the environment, i.e., in the physical world. They are the starting point of each measurement as they act as triggers for sensors.

They can also be actively produced by a sensor to perform observations about real physical world . The same types of stimulus can trigger different kinds of sensors and be used to reason about different properties. 

ex: In biology, a stimulus is a change in an organism's surroundings that causes the organism to change its behavior in order to make the environment more satisfactory. For instance, 1- hunger motivates animals to seek food, 2- predators stimulate prey to run away or hide, and 3- falling temperatures encourage creatures to seek shelter or find warmth in other ways""" ;
	rdfs:isDefinedBy "http://purl.oclc.org/NET/ssnx/ssn" ;
	rdfs:label "Stimulus" ;
	rdfs:seeAlso "http://www.w3.org/2005/Incubator/ssn/wiki/SSN_Skeleton#Skeleton" .
# 
# http://purl.oclc.org/NET/ssnx/ssn#SurvivalProperty

ssn:SurvivalProperty a owl:Class ;
	rdfs:subClassOf ssn:Property ;
	rdfs:comment "An identifiable characteristic that represents the extent of the sensors useful life.  Might include for example total battery life or number of recharges, or, for sensors that are used only a fixed number of times, the number of observations that can be made before the sensing capability is depleted." ;
	rdfs:isDefinedBy "http://purl.oclc.org/NET/ssnx/ssn" ;
	rdfs:label "Survival Property" ;
	rdfs:seeAlso "http://www.w3.org/2005/Incubator/ssn/wiki/SSN_Deploy#OperatingRestriction" .
# 
# http://purl.oclc.org/NET/ssnx/ssn#SurvivalRange

ssn:SurvivalRange a owl:Class ;
	rdfs:subClassOf ssn:Property , _:genid30 .

_:genid30 a owl:Restriction ;
	owl:onProperty ssn:hasSurvivalProperty ;
	owl:allValuesFrom ssn:SurvivalProperty .

ssn:SurvivalRange rdfs:subClassOf _:genid31 .

_:genid31 a owl:Restriction ;
	owl:onProperty ssn:inCondition ;
	owl:allValuesFrom ssn:Condition .

ssn:SurvivalRange rdfs:comment "The conditions a sensor can be exposed to without damage: i.e., the sensor continues to operate as defined using MeasurementCapability.  If, however, the SurvivalRange is exceeded, the sensor is 'damaged' and MeasurementCapability specifications may no longer hold." ;
	rdfs:isDefinedBy "http://purl.oclc.org/NET/ssnx/ssn" ;
	rdfs:label "Survival Range" ;
	rdfs:seeAlso "http://www.w3.org/2005/Incubator/ssn/wiki/SSN_Deploy#OperatingRestriction" .
# 
# http://purl.oclc.org/NET/ssnx/ssn#System

ssn:System a owl:Class ;
	rdfs:subClassOf _:genid32 .

_:genid32 a owl:Restriction ;
	owl:onProperty ssn:hasSubSystem ;
	owl:someValuesFrom ssn:System .

ssn:System rdfs:subClassOf _:genid33 .

_:genid33 a owl:Restriction ;
	owl:onProperty ssn:hasDeployment ;
	owl:allValuesFrom ssn:Deployment .

ssn:System rdfs:subClassOf _:genid34 .

_:genid34 a owl:Restriction ;
	owl:onProperty ssn:hasOperatingRange ;
	owl:allValuesFrom ssn:OperatingRange .

ssn:System rdfs:subClassOf _:genid35 .

_:genid35 a owl:Restriction ;
	owl:onProperty ssn:hasSubSystem ;
	owl:allValuesFrom ssn:System .

ssn:System rdfs:subClassOf _:genid36 .

_:genid36 a owl:Restriction ;
	owl:onProperty ssn:hasSurvivalRange ;
	owl:allValuesFrom ssn:SurvivalRange .

ssn:System rdfs:subClassOf _:genid37 .

_:genid37 a owl:Restriction ;
	owl:onProperty ssn:onPlatform ;
	owl:allValuesFrom ssn:Platform .

ssn:System rdfs:comment "System is a unit of abstraction for pieces of infrastructure (and we largely care that they are) for sensing. A system has components, its subsystems, which are other systems." ;
	rdfs:isDefinedBy "http://purl.oclc.org/NET/ssnx/ssn" ;
	rdfs:label "System" ;
	rdfs:seeAlso "http://www.w3.org/2005/Incubator/ssn/wiki/SSN_Model#System" .
# 
# http://purl.oclc.org/NET/ssnx/ssn#SystemLifetime

ssn:SystemLifetime a owl:Class ;
	rdfs:subClassOf ssn:SurvivalProperty ;
	rdfs:comment "Total useful life of a sensor/system (expressed as total life since manufacture, time in use, number of operations, etc.)." ;
	rdfs:isDefinedBy "http://purl.oclc.org/NET/ssnx/ssn" ;
	rdfs:label "System Lifetime" ;
	rdfs:seeAlso "http://www.w3.org/2005/Incubator/ssn/wiki/SSN_Deploy#OperatingRestriction" .
# 
# http://purl.org/NET/ssnx/qu/qu#QuantityKind

qu:QuantityKind a owl:Class ;
	rdfs:comment """A QuantityKind is an abstract classifier that represents the [VIM] concept of \"kind of quantity\" that is defined as \"aspect common to mutually comparable quantities.\" A QuantityKind represents the essence of a quantity without any numerical value or unit.  

eg: Tempreture Sensor hasQuantityKind tempreture(instance from QuantityKind Class)""" ;
	rdfs:label "Quantity Kind" .
# 
# http://purl.org/NET/ssnx/qu/qu#Unit

qu:Unit a owl:Class ;
	rdfs:comment "Unit of measurement . ex: microAmpere" .
# 
# http://www.w3.org/2000/01/rdf-schema#Class

rdfs:Class a owl:Class .
# 
# http://www.w3.org/2002/07/owl#Thing

owl:Thing rdfs:label "Thing" .
# 
# http://www.w3.org/2003/01/geo/wgs84_pos#Point

geo:Point a owl:Class ;
	rdfs:comment """ 
Uniquely identified by lat/long/alt. i.e.

spaciallyIntersects(P1, P2) :- lat(P1, LAT), long(P1, LONG), alt(P1, ALT),
  lat(P2, LAT), long(P2, LONG), alt(P2, ALT).

sameThing(P1, P2) :- type(P1, Point), type(P2, Point), spaciallyIntersects(P1, P2).
  """ , """A point, typically described using a coordinate system relative to Earth, such as WGS84.
  
Ex: <geo:Point>
           <geo:lat>55.701</geo:lat>
           <geo:long>12.552</geo:long>
      </geo:Point>""" ;
	rdfs:label "point" .
# 
# http://xmlns.com/foaf/0.1/Agent

foaf:Agent a owl:Class ;
	rdfs:comment "An agent (eg. person, group, software or physical artifact)." ;
	rdfs:label "Agent" ;
	<http://www.w3.org/2003/06/sw-vocab-status/ns#term_status> "stable" .
# 
# http://xmlns.com/foaf/0.1/Group

foaf:Group a owl:Class ;
	rdfs:subClassOf foaf:Agent ;
	rdfs:comment "A class of Agents." ;
	rdfs:label "Group" ;
	<http://www.w3.org/2003/06/sw-vocab-status/ns#term_status> "stable" .
# 
# http://xmlns.com/foaf/0.1/Organization

foaf:Organization a owl:Class ;
	rdfs:subClassOf foaf:Agent ;
	owl:disjointWith foaf:Person ;
	rdfs:comment "An organization." ;
	rdfs:isDefinedBy <http://xmlns.com/foaf/0.1/> ;
	rdfs:label "Organization" ;
	<http://www.w3.org/2003/06/sw-vocab-status/ns#term_status> "stable" .
# 
# http://xmlns.com/foaf/0.1/Person

foaf:Person a owl:Class ;
	rdfs:subClassOf foaf:Agent ;
	rdfs:comment "A person." ;
	rdfs:isDefinedBy <http://xmlns.com/foaf/0.1/> ;
	rdfs:label "Person" ;
	<http://www.w3.org/2003/06/sw-vocab-status/ns#term_status> "stable" .
# 
# 
# 
# #################################################################
# #
# #    Annotations
# #
# #################################################################
# 
# 

<http://www.w3.org/2003/01/geo/wgs84_pos#> rdfs:label "geo" ;
	rdfs:comment """
Recent changes to this namespace:
$Log: wgs84_pos.rdf,v $
Revision 1.22  2009/04/20 15:00:30  timbl
Remove the time bits which have been deal with elsewhere eg in iCal.

Revision 1.21  2009/04/20 12:52:47  timbl
try again

Revision 1.20  2009/04/20 12:42:11  timbl
Add Event (edited ages ago and never checked in), and location (following discussion http://chatlogs.planetrdf.com/swig/2009-04-20#T12-36-09)

Revision 1.19  2009/04/20 12:36:31  timbl
Add Event (edited ages ago and never checked in), and location (following discussion http://chatlogs.planetrdf.com/swig/2009-04-20#T12-36-09)

Revision 1.18  2006/02/01 22:01:04  danbri
Clarified that lat and long are decimal degrees, and that alt is decimal metres about local reference ellipsoid

Revision 1.17  2004/02/06 17:38:12  danbri
Fixed a bad commit screwup

Revision 1.15  2003/04/19 11:24:08  danbri
Fixed the typo even more.

Revision 1.14  2003/04/19 11:16:56  danbri
fixed a typo

Revision 1.13  2003/02/19 22:27:27  connolly
relaxed domain constraints on lat/long/alt from Point to SpatialThing

Revision 1.12  2003/01/12 01:41:41  danbri
Trying local copy of XSLT doc.

Revision 1.11  2003/01/12 01:20:18  danbri
added a link to morten's xslt rdfs viewer.

Revision 1.10  2003/01/11 18:56:49  danbri
Removed datatype range from lat and long properties, since they would
have required each occurance of the property to mention the datatype.

Revision 1.9  2003/01/11 11:41:31  danbri
Another typo; repaired rdfs:Property to rdf:Property x4

Revision 1.8  2003/01/11 11:05:02  danbri
Added an rdfs:range for each lat/long/alt property,
http://www.w3.org/2001/XMLSchema#float

Revision 1.7  2003/01/10 20:25:16  danbri
Longer rdfs:comment for Point, trying to be Earth-centric and neutral about
coordinate system(s) at the same time. Feedback welcomed.

Revision 1.6  2003/01/10 20:18:30  danbri
Added CVS log comments into the RDF/XML as an rdfs:comment property of the
vocabulary. Note that this is not common practice (but seems both harmless
and potentially useful).


revision 1.5
date: 2003/01/10 20:14:31;  author: danbri;  state: Exp;  lines: +16 -5
Updated schema:
Added a dc:date, added url for more info. Changed the rdfs:label of the
namespace from gp to geo. Added a class Point, set as the rdfs:domain of
each property. Added XML comment on the lat_long property suggesting that
we might not need it (based on #rdfig commentary from implementors).

revision 1.4
date: 2003/01/10 20:01:07;  author: danbri;  state: Exp;  lines: +6 -5
Fixed typo; several rdfs:about attributes are now rdf:about. Thanks to MortenF in
#rdfig for catching this error.

revision 1.3
date: 2003/01/10 11:59:03;  author: danbri;  state: Exp;  lines: +4 -3
fixed buglet in vocab, added more wgs links

revision 1.2
date: 2003/01/10 11:01:11;  author: danbri;  state: Exp;  lines: +4 -4
Removed alt from the as-a-flat-string property, and switched from
space separated to comma separated.

revision 1.1
date: 2003/01/10 10:53:23;  author: danbri;  state: Exp;
basic geo vocab

""" .
# 

geo:lat_long rdfs:comment "A comma-separated representation of a latitude, longitude coordinate." ;
	rdfs:label "lat/long" .
# 
# Generated by the OWL API (version 4.2.6.20160910-2108) https://github.com/owlcs/owlapi
